src/Run.v
@@ -1,10 +1,8 @@
 Require Import Coq.ZArith.BinInt.
 Require Import coqutil.Word.LittleEndian.
-Require Import riscv.util.BitWidths.
 Require Import riscv.util.Monads.
 Require Import riscv.util.MonadNotations.
 Require Import riscv.Decode.
-Require Import riscv.util.BitWidths.
 Require Import riscv.Memory. (* should go before Program because both define loadByte etc *)
 Require Import riscv.Program.
 Require Import riscv.Execute.
@@ -13,7 +11,6 @@ Require Import riscv.Utility.
 
 Section Riscv.
 
-  Context {B: BitWidths}.
   Context {mword: Type}.
   Context {MW: MachineWidth mword}.
 
@@ -22,20 +19,14 @@ Section Riscv.
   Context {RVP: RiscvProgram M mword}.
   Context {RVS: RiscvState M mword}.
 
-  Definition RV_wXLEN_IM: InstructionSet :=
-    match bitwidth with
-    | BW32 => RV32IM
-    | BW64 => RV64IM
-    end.
-
-  Definition run1:
+  Definition run1(iset: InstructionSet):
     M unit :=
     pc <- getPC;
     inst <- loadWord pc;
-    execute (decode RV_wXLEN_IM (combine 4 inst));;
+    execute (decode iset (combine 4 inst));;
     step.
 
-  Definition run: nat -> M unit :=
-    fun n => power_func (fun m => run1 ;; m) n (Return tt).
+  Definition run(iset: InstructionSet)(n: nat): M unit :=
+    power_func (fun m => run1 iset;; m) n (Return tt).
 
 End Riscv.
