src/MinimalMMIO.v
@@ -1,7 +1,6 @@
 Require Import Coq.ZArith.ZArith.
 Require Import Coq.Logic.FunctionalExtensionality.
 Require Import Coq.Logic.PropExtensionality.
-Require Import riscv.util.BitWidths.
 Require Import riscv.util.Monads. Import OStateNDOperations.
 Require Import riscv.util.MonadNotations.
 Require Import riscv.Decode.
