src/util/BitWidth32.v
@@ -1,3 +1,0 @@
-Require Import riscv.util.BitWidths.
-
-Instance BitWidth32: BitWidths := BW32.
